\chapter{积分表}
\def\mysec#1{\section*{含有\(#1\)的积分}}
\begin{enumerate}
\mysec{ax+b}
\item \(\int \frac{\dd{x}}{ax+b} = \frac{1}{a} \ln\abs{ax+b} + C\)

\item \(\int (ax+b)^{\mu} \dd{x} = \frac{1}{a(\mu+1)} (ax+b)^{\mu+1} + C\ (\mu\neq-1)\)

\item \(\int \frac{x}{ax+b} \dd{x} = \frac{1}{a^2} (ax+b-b\ln\abs{ax+b}) + C\)

\item \(\int \frac{x^2}{ax+b} \dd{x} = \frac{1}{a^3} \left[
	\frac{1}{2} (ax+b)^2 - 2b(ax+b) + b^2 \ln\abs{ax+b}
\right] + C\)

\item \(\int \frac{\dd{x}}{x(ax+b)} = -\frac{1}{b} \ln\abs{\frac{ax+b}{x}} + C\)

\item \(\int \frac{\dd{x}}{x^2(ax+b)} = -\frac{1}{bx} + \frac{a}{b^2} \ln\abs{\frac{ax+b}{x}} + C\)

\item \(\int \frac{x\dd{x}}{(ax+b)^2} = \frac{1}{a^2} \left( \ln\abs{ax+b} + \frac{b}{ax+b} \right) + C\)

\item \(\int \frac{x^2 \dd{x}}{(ax+b)^2} = \frac{1}{a^3} \left( ax+b - 2b \ln\abs{ax+b} - \frac{b^2}{ax+b} \right) + C\)

\item \(\int \frac{\dd{x}}{x(ax+b)^2} = \frac{1}{b(ax+b)} - \frac{1}{b^2} \ln\abs{\frac{ax+b}{x}} + C\)

\mysec{\sqrt{ax+b}}
\item \(\int \sqrt{ax+b} \dd{x} = \frac{2}{3a} \sqrt{ax+b}^3 + C\)

\item \(\int x \sqrt{ax+b} \dd{x} = \frac{2}{15a^2} (3ax-2b) \sqrt{ax+b}^3 + C\)

\item \(\int x^2 \sqrt{ax+b} \dd{x} = \frac{2}{105a^3} (15a^2x^2-12abx+8b^2) \sqrt{ax+b}^3 + C\)

\item \(\int \frac{x \dd{x}}{\sqrt{ax+b}} = \frac{2}{3a^2} (ax-2b) \sqrt{ax+b} + C\)

\item \(\int \frac{x^2 \dd{x}}{\sqrt{ax+b}} = \frac{2}{15a^3} (3a^2x^2-4abx+8b^2) \sqrt{ax+b} + C\)

\item \(\int \frac{\dd{x}}{x \sqrt{ax+b}} = \left\{ \begin{array}{lc}
\frac{1}{\sqrt{b}} \ln\abs{\frac{\sqrt{ax+b}-\sqrt{b}}{\sqrt{ax+b}+\sqrt{b}}} + C, & b>0, \\
\frac{2}{\sqrt{-b}} \arctan\sqrt{\frac{ax+b}{-b}} + C, & b<0
\end{array} \right.\)

\item \(\int \frac{\dd{x}}{x^2 \sqrt{ax+b}} = -\frac{\sqrt{ax+b}}{bx} - \frac{a}{2b} \int \frac{\dd{x}}{x \sqrt{ax+b}}\)

\item \(\int \frac{\sqrt{ax+b}}{x} \dd{x} = 2\sqrt{ax+b} + b \int \frac{\dd{x}}{x \sqrt{ax+b}}\)

\item \(\int \frac{\sqrt{ax+b}}{x^2} \dd{x} = -\frac{\sqrt{ax+b}}{x} + \frac{a}{2} \int \frac{\dd{x}}{x \sqrt{ax+b}}\)

\mysec{x^2 \pm a^2}
\item \(\int \frac{\dd{x}}{x^2+a^2} = \frac{1}{a} \arctan\frac{x}{a} + C\)

\item \(\int \frac{\dd{x}}{(x^2+a^2)^n} = \frac{x}{2(n-1)a^2(x^2+a^2)^{n-1}} + \frac{2n-3}{2(n-1)a^2} \int \frac{\dd{x}}{(x^2+a^2)^{n-1}}\)

\item \(\int \frac{\dd{x}}{x^2-a^2} = \frac{1}{2a} \ln\abs{\frac{x-a}{x+a}} + C\)

\mysec{ax^2+b\ (a>0)}
\item \(\int \frac{\dd{x}}{ax^2+b} = \left\{ \begin{array}{ll}
\frac{1}{\sqrt{ab}} \arctan\sqrt{\frac{a}{b}}x + C, & b>0, \\
\frac{1}{2\sqrt{-ab}} \ln\abs{\frac{\sqrt{a}x - \sqrt{-b}}{\sqrt{a}x + \sqrt{-b}}} + C, & b<0
\end{array} \right.\)

\item \(\int \frac{x \dd{x}}{ax^2+b} = \frac{1}{2a} \ln\abs{ax^2+b} + C\)

\item \(\int \frac{x^2 \dd{x}}{ax^2+b} = \frac{x}{a} - \frac{b}{a} \int \frac{\dd{x}}{ax^2+b}\)

\item \(\int \frac{\dd{x}}{x(ax^2+b)} = \frac{1}{2b} \ln\frac{x^2}{\abs{ax^2+b}} + C\)

\item \(\int \frac{\dd{x}}{x^2(ax^2+b)} = -\frac{1}{bx} - \frac{a}{b} \int \frac{\dd{x}}{ax^2+b}\)

\item \(\int \frac{\dd{x}}{x^3(ax^2+b)} = \frac{a}{2b^2} \ln\frac{\abs{ax^2+b}}{x^2} - \frac{1}{2bx^2} + C\)

\item \(\int \frac{\dd{x}}{(ax^2+b)^2} = \frac{x}{2b(ax^2+b)} + \frac{1}{2b} \int \frac{\dd{x}}{ax^2+b}\)

\mysec{ax^2+bx+c\ (a>0)}
\item \(\int \frac{\dd{x}}{ax^2+bx+c} = \left\{ \begin{array}{ll}
\frac{2}{\sqrt{4ac-b^2}} \arctan\frac{2ax+b}{\sqrt{4ac-b^2}} + C, & b^2<4ac, \\
\frac{1}{\sqrt{b^2-4ac}} \ln\abs{\frac{2ax+b-\sqrt{b^2-4ac}}{2ax+b+\sqrt{b^2-4ac}}} + C, & b^2>4ac
\end{array} \right.\)

\item \(\int \frac{x \dd{x}}{ax^2+bx+c} = \frac{1}{2a} \ln\abs{ax^2+bx+c} - \frac{b}{2a} \int \frac{\dd{x}}{ax^2+bx+c}\)

\mysec{\sqrt{x^2+a^2}\ (a>0)}
\item \(\int \frac{\dd{x}}{\sqrt{x^2+a^2}} = \arsinh\frac{x}{a} + C_1
= \ln(x+\sqrt{x^2+a^2}) + C\)

\item \(\int \frac{\dd{x}}{\sqrt{x^2+a^2}^3} = \frac{x}{a^2 \sqrt{x^2+a^2}} + C\)

\item \(\int \frac{x \dd{x}}{\sqrt{x^2+a^2}} = \sqrt{x^2+a^2} + C\)

\item \(\int \frac{x \dd{x}}{\sqrt{x^2+a^2}^3} = -\frac{1}{\sqrt{x^2+a^2}} + C\)

\item \(\int \frac{x^2 \dd{x}}{\sqrt{x^2+a^2}} = \frac{x}{2}\sqrt{x^2+a^2} - \frac{a^2}{2} \ln(x+\sqrt{x^2+a^2}) + C\)

\item \(\int \frac{x^2 \dd{x}}{\sqrt{x^2+a^2}^3} = -\frac{x}{\sqrt{x^2+a^2}} + \ln(x+\sqrt{x^2+a^2}) + C\)

\item \(\int \frac{\dd{x}}{x\sqrt{x^2+a^2}} = \frac{1}{a} \ln\frac{\sqrt{x^2+a^2}-a}{\abs{x}} + C\)

\item \(\int \frac{\dd{x}}{x^2\sqrt{x^2+a^2}} = -\frac{\sqrt{x^2+a^2}}{a^2 x} + C\)

\item \(\int \sqrt{x^2+a^2} \dd{x} = \frac{x}{2} \sqrt{x^2+a^2} + \frac{a^2}{2} \ln(x+\sqrt{x^2+a^2}) + C\)

\item \(\int \sqrt{x^2+a^2}^3 \dd{x} = \frac{x}{8} (2x^2+5a^2) \sqrt{x^2+a^2} + \frac{3}{8} a^4 \ln(x+\sqrt{x^2+a^2}) + C\)

\item \(\int x\sqrt{x^2+a^2} \dd{x} = \frac{1}{3} \sqrt{x^2+a^2}^3 + C\)

\item \(\int x^2\sqrt{x^2+a^2} \dd{x} = \frac{x}{8} (2x^2+a^2) \sqrt{x^2+a^2} - \frac{a^4}{8} \ln(x+\sqrt{x^2+a^2}) + C\)

\item \(\int \frac{\sqrt{x^2+a^2}}{x} \dd{x} = \sqrt{x^2+a^2} + a\ln\frac{\sqrt{x^2+a^2}-a}{\abs{x}} + C\)

\item \(\int \frac{\sqrt{x^2+a^2}}{x^2} \dd{x} = -\frac{\sqrt{x^2+a^2}}{x} + \ln(x+\sqrt{x^2+a^2}) + C\)

\mysec{\sqrt{x^2-a^2}\ (a>0)}
\item \(\int \frac{\dd{x}}{\sqrt{x^2-a^2}} = \frac{x}{\abs{x}} \arcosh\frac{\abs{x}}{a} + C_1
= \ln\abs{x+\sqrt{x^2-a^2}} + C\)

\item \(\int \frac{\dd{x}}{\sqrt{x^2-a^2}^3} = -\frac{x}{a^2\sqrt{x^2-a^2}} + C\)

\item \(\int \frac{x \dd{x}}{\sqrt{x^2-a^2}} = \sqrt{x^2-a^2} + C\)

\item \(\int \frac{x \dd{x}}{\sqrt{x^2-a^2}^3} = -\frac{1}{\sqrt{x^2-a^2}} + C\)

\item \(\int \frac{x^2 \dd{x}}{\sqrt{x^2-a^2}} = \frac{x}{2} \sqrt{x^2-a^2} + \frac{a^2}{2} \ln\abs{x+\sqrt{x^2-a^2}} + C\)

\item \(\int \frac{x^2 \dd{x}}{\sqrt{x^2-a^2}^3} = -\frac{x}{\sqrt{x^2-a^2}} + \ln\abs{x+\sqrt{x^2-a^2}} + C\)

\item \(\int \frac{\dd{x}}{x\sqrt{x^2-a^2}} = \frac{1}{a} \arccos\frac{a}{\abs{x}} + C\)

\item \(\int \frac{\dd{x}}{x^2\sqrt{x^2-a^2}} = \frac{\sqrt{x^2-a^2}}{a^2 x} + C\)

\item \(\int \sqrt{x^2-a^2} \dd{x} = \frac{x}{2} \sqrt{x^2-a^2} - \frac{a^2}{2} \ln\abs{x+\sqrt{x^2-a^2}} + C\)

\item \(\int \sqrt{x^2-a^2}^3 \dd{x} = \frac{x}{8} (2x^2-5a^2) \sqrt{x^2-a^2} + \frac{3}{8} a^4 \ln\abs{x+\sqrt{x^2-a^2}} + C\)

\item \(\int x\sqrt{x^2-a^2} \dd{x} = \frac{1}{3} \sqrt{x^2-a^2}^3 + C\)

\item \(\int x^2 \sqrt{x^2-a^2} \dd{x} = \frac{x}{8} (2x^2-a^2) \sqrt{x^2-a^2} - \frac{a^4}{8} \ln\abs{x+\sqrt{x^2-a^2}} + C\)

\item \(\int \frac{\sqrt{x^2-a^2}}{x} \dd{x} = \sqrt{x^2-a^2} - a \arccos\frac{a}{\abs{x}} + C\)

\item \(\int \frac{\sqrt{x^2-a^2}}{x^2} \dd{x} = -\frac{\sqrt{x^2-a^2}}{x} + \ln\abs{x+\sqrt{x^2-a^2}} + C\)

\mysec{\sqrt{a^2-x^2}\ (a>0)}
\item \(\int \frac{\dd{x}}{\sqrt{a^2-x^2}} = \arcsin\frac{x}{a} + C\)
\item \(\int \frac{\dd{x}}{\sqrt{(a^2-x^2)^3}} = \frac{x}{a^2 \sqrt{a^2-x^2}} + C\)
\item \(\int \frac{x}{\sqrt{a^2-x^2}} \dd{x} = -\sqrt{a^2-x^2} + C\)
\item \(\int \frac{x}{\sqrt{(a^2-x^2)^3}} \dd{x} = \frac{1}{\sqrt{a^2-x^2}} + C\)
\item \(\int \frac{x^2}{\sqrt{a^2-x^2}} \dd{x} = -\frac{x}{2} \sqrt{a^2-x^2} + \frac{a^2}{2} \arcsin\frac{x}{a} + C\)
\item \(\int \frac{x^2}{\sqrt{(a^2-x^2)^3}} \dd{x} = \frac{x}{\sqrt{a^2-x^2}} - \arcsin\frac{x}{a} + C\)
\item \(\int \frac{\dd{x}}{x \sqrt{a^2-x^2}} = \frac{1}{a} \ln\frac{a-\sqrt{a^2-x^2}}{\abs{x}} + C\)
\item \(\int \frac{\dd{x}}{x^2 \sqrt{a^2-x^2}} = -\frac{\sqrt{a^2-x^2}}{a^2 x} + C\)
\item \(\int \sqrt{a^2-x^2} \dd{x} = \frac{x}{2} \sqrt{a^2-x^2} + \frac{a^2}{2} \arcsin\frac{x}{a} + C\)
\item \(\int \sqrt{(a^2-x^2)^3} \dd{x} = \frac{x}{8} (5a^2 - 2x^2) \sqrt{a^2-x^2} + \frac{3}{8} a^4 \arcsin\frac{x}{a} + C\)
\item \(\int x \sqrt{a^2-x^2} \dd{x} = -\frac{1}{3} \sqrt{(a^2-x^2)^3} + C\)
\item \(\int x^2 \sqrt{a^2-x^2} \dd{x} = \frac{x}{8} (2x^2 - a^2) \sqrt{a^2-x^2} + \frac{a^4}{8} \arcsin\frac{x}{a} + C\)
\item \(\int \frac{\sqrt{a^2-x^2}}{x} \dd{x} = \sqrt{a^2-x^2} + a \ln\frac{a-\sqrt{a^2-x^2}}{\abs{x}} + C\)
\item \(\int \frac{\sqrt{a^2-x^2}}{x^2} \dd{x} = -\frac{\sqrt{a^2-x^2}}{x} - \arcsin\frac{x}{a} + C\)

\mysec{\sqrt{\pm ax^2+bx+c}\ (a>0)}
\item \(\int \frac{\dd{x}}{\sqrt{ax^2+bx+c}} = \frac{1}{\sqrt{a}} \ln\abs{2ax+b+2\sqrt{a}\sqrt{ax^2+bx+c}} + C\)
\item \(\begin{aligned}[t]
\int \sqrt{ax^2+bx+c} \dd{x}
&= \frac{2ax+b}{4a} \sqrt{ax^2+bx+c} \\
&\hspace{20pt}+ \frac{4ac-b^2}{8\sqrt{a^3}} \ln\abs{2ax+b+2\sqrt{a}\sqrt{ax^2+bx+c}} + C
\end{aligned}\)
\item \(\begin{aligned}[t]
\int \frac{x}{\sqrt{ax^2+bx+c}} \dd{x}
&= \frac{1}{a}\sqrt{ax^2+bx+c} \\
&\hspace{20pt}- \frac{b}{2\sqrt{a^3}} \ln\abs{2ax+b+2\sqrt{a}\sqrt{ax^2+bx+c}} + C
\end{aligned}\)
\item \(\int \frac{\dd{x}}{\sqrt{c+bx-ax^2}} = -\frac{1}{\sqrt{a}} \arcsin\frac{2ax-b}{\sqrt{b^2+4ac}} + C\)
\item \(\int \sqrt{c+bx-ax^2} \dd{x} = \frac{2ax-b}{4a} \sqrt{c+bx-ax^2} + \frac{b^2+4ac}{8\sqrt{a^3}} \arcsin\frac{2ax-b}{b^2+4ac} + C\)
\item \(\int \frac{x}{\sqrt{c+bx-ax^2}} \dd{x} = -\frac{1}{a} \sqrt{c+bx-ax^2} + \frac{b}{2\sqrt{a^3}} \arcsin\frac{2ax-b}{b^2+4ac} + C\)

\section*{含有\(\sqrt{\pm\frac{x-a}{x-b}}\)或\(\sqrt{(x-a)(b-x)}\)的积分}
\item \(\int \sqrt{\frac{x-a}{x-b}} \dd{x} = (x-b) \sqrt{\frac{x-a}{x-b}} + (b-a) \ln(\sqrt{\abs{x-a}} + \sqrt{\abs{x-b}}) + C\)
\item \(\int \sqrt{\frac{x-a}{b-x}} \dd{x} = (x-b) \sqrt{\frac{x-a}{b-x}} + (b-a) \arcsin\sqrt{\frac{x-a}{b-x}} + C\)
\item \(\int \frac{\dd{x}}{\sqrt{(x-a)(b-x)}} = 2\arcsin\sqrt{\frac{x-a}{b-a}} + C \quad(a<b)\)
\item \(\begin{aligned}[t]
\int \sqrt{(x-a)(b-x)} \dd{x}
&= \frac{2x-a-b}{4} \sqrt{(x-a)(b-x)} \\
&\hspace{20pt}+ \frac{(b-a)^2}{4} \arcsin\sqrt{\frac{x-a}{b-a}} + C \quad(a<b)
\end{aligned}\)

\section*{含有三角函数的积分}
\item \(\int \sin x \dd{x}
= -\cos x + C\)
\item \(\int \cos x \dd{x}
= \sin x + C\)
\item \(\int \tan x \dd{x}
= -\ln\abs{\cos x} + C\)
\item \(\int \cot x \dd{x}
= \ln\abs{\sin x} + C\)
\item \(\begin{aligned}[t]
\int \sec x \dd{x}
&= \ln\abs{\tan\left(\frac{\pi}{4}+\frac{x}{2}\right)} + C \\
&= \ln\abs{\sec x + \tan x} + C
\end{aligned}\)
\item \(\begin{aligned}[t]
\int \csc x \dd{x}
&= \ln\abs{\tan \frac{x}{2}} + C \\
&= \ln\abs{\csc x - \cot x} + C
\end{aligned}\)
\item \(\int \sec^2 x \dd{x} = \tan x + C\)
\item \(\int \csc^2 x \dd{x} = -\cot x + C\)
\item \(\int \sec x \tan x \dd{x} = \sec x + C\)
\item \(\int \csc x \cot x \dd{x} = -\csc x + C\)
\item \(\int \sin^2 x \dd{x} = \frac{x}{2} - \frac{1}{4} \sin 2x + C\)
\item \(\int \cos^2 x \dd{x} = \frac{x}{2} + \frac{1}{4} \sin 2x + C\)
\item \(\int \sin^n x \dd{x} = -\frac{1}{n} \sin^{n-1} x \cos x + \frac{n-1}{n} \int \sin^{n-2} x \dd{x}\)
\item \(\int \cos^n x \dd{x} = \frac{1}{n} \cos^{n-1} x \sin x + \frac{n-1}{n} \int \cos^{n-2} x \dd{x}\)
\item \(\int \frac{\dd{x}}{\sin^n x} = -\frac{1}{n-1}\cdot\frac{\cos x}{\sin^{n-1} x} + \frac{n-2}{n-1} \int \frac{\dd{x}}{\sin^{n-2} x}\)
\item \(\int \frac{\dd{x}}{\cos^n x} = \frac{1}{n-1}\cdot\frac{\sin x}{\cos^{n-1} x} + \frac{n-2}{n-1} \int \frac{\dd{x}}{\cos^{n-2} x}\)
\item \(\begin{aligned}[t]
\int \cos^m x \sin^n x \dd{x}
&= \frac{1}{m+n} \cos^{m-1} x \sin^{n+1} x + \frac{m-1}{m+n} \int \cos^{m-2} x \sin^n x \dd{x} \\
&= -\frac{1}{m+n} \cos^{m+1} x \sin^{n-1} x + \frac{n-1}{m+n} \int \cos^m x \sin^{n-2} x \dd{x}
\end{aligned}\)
\item \(\int \sin ax \cos bx \dd{x}
= -\frac{1}{2(a+b)} \cos(a+b)x - \frac{1}{2(a-b)} \cos(a-b)x + C\)
\item \(\int \sin ax \sin bx \dd{x} = -\frac{1}{2(a+b)} \sin(a+b)x + \frac{1}{2(a-b)} \sin(a-b)x + C\)
\item \(\int \cos ax \cos bx \dd{x} = \frac{1}{2(a+b)} \sin(a+b)x + \frac{1}{2(a-b)} \sin(a-b)x + C\)
\item \(\int \frac{\dd{x}}{a+b\sin x} = \frac{2}{\sqrt{a^2-b^2}} \arctan\frac{a\tan\frac{x}{2}+b}{\sqrt{a^2-b^2}} + C\ (a^2>b^2)\)
\item \(\int \frac{\dd{x}}{a+b\sin x} = \frac{1}{\sqrt{b^2-a^2}} \ln\abs{\frac{a\tan\frac{x}{2}+b-\sqrt{b^2-a^2}}{a\tan\frac{x}{2}+b+\sqrt{b^2-a^2}}} + C\ (a^2<b^2)\)
\item \(\int \frac{\dd{x}}{a+b\cos x} = \frac{2}{a+b} \sqrt{\frac{a+b}{a-b}} \arctan\left(\sqrt{\frac{a-b}{a+b}} \tan\frac{x}{2}\right) + C\ (a^2>b^2)\)
\item \(\int \frac{\dd{x}}{a+b\cos x} = \frac{1}{a+b} \sqrt{\frac{a+b}{a-b}} \ln\abs{\frac{\tan\frac{x}{2}+\sqrt{\frac{a+b}{b-a}}}{\tan\frac{x}{2}-\sqrt{\frac{a+b}{b-a}}}} + C\ (a^2<b^2)\)
\item \(\int \frac{\dd{x}}{a^2\cos^2 x+b^2\sin^2 x} = \frac{1}{ab} \arctan\left(\frac{b}{a} \tan x\right) + C\)
\item \(\int \frac{\dd{x}}{a^2\cos^2 x-b^2\sin^2 x} = \frac{1}{2ab} \ln\abs{\frac{b\tan x + a}{b\tan x - a}} + C\)
\item \(\int x \sin ax \dd{x} = \frac{1}{a^2} \sin ax - \frac{1}{a} x \cos ax + C\)
\item \(\int x^2 \sin ax \dd{x} = -\frac{1}{a}x^2\cos ax + \frac{2}{a^2} x\sin ax + \frac{2}{a^3} \cos ax + C\)
\item \(\int x \cos ax \dd{x} = \frac{1}{a^2} \cos ax + \frac{1}{a} x \sin ax + C\)
\item \(\int x^2 \cos ax \dd{x} = \frac{1}{a} x^2 \sin ax + \frac{2}{a^2} x \cos ax - \frac{2}{a^3} \sin ax + C\)

\section*{含有反三角函数的积分\texorpdfstring{（其中\(a>0\)）}{}}
\item \(\int \arcsin\frac{x}{a} \dd{x}
= x \arcsin\frac{x}{a} + \sqrt{a^2-x^2} + C\)
\item \(\int x \arcsin\frac{x}{a} \dd{x}
= \left(\frac{x^2}{2}-\frac{a^2}{4}\right) \arcsin\frac{x}{a}
+ \frac{x}{4} \sqrt{a^2-x^2} + C\)
\item \(\int x^2 \arcsin\frac{x}{a} \dd{x}
= \frac{x^3}{3} \arcsin\frac{x}{a}
+ \frac{1}{9} (x^2+2a^2) \sqrt{a^2-x^2} + C\)
\item \(\int \arccos\frac{x}{a} \dd{x}
= x \arccos\frac{x}{a} - \sqrt{a^2-x^2} + C\)
\item \(\int x \arccos\frac{x}{a} \dd{x}
= \left(\frac{x^2}{2}-\frac{a^2}{4}\right) \arccos\frac{x}{a}
- \frac{x}{4} \sqrt{a^2-x^2} + C\)
\item \(\int x^2 \arccos\frac{x}{a} \dd{x}
= \frac{x^3}{3} \arccos\frac{x}{a}
- \frac{1}{9} (x^2+2a^2) \sqrt{a^2-x^2} + C\)
\item \(\int \arctan\frac{x}{a} \dd{x}
= x \arctan\frac{x}{a} - \frac{a}{2} \ln(a^2+x^2) + C\)
\item \(\int x \arctan\frac{x}{a} \dd{x}
= \frac{1}{2} (a^2+x^2) \arctan\frac{x}{a} - \frac{a}{2} x + C\)
\item \(\int x^2 \arctan\frac{x}{a} \dd{x}
= \frac{x^3}{3} \arctan\frac{x}{a}
- \frac{a}{6} x^2 + \frac{a^3}{6} \ln(a^2+x^2) + C\)

\section*{含有指数函数的积分}
\item \(\int a^x \dd{x} = \frac{1}{\ln a} a^x + C\)
\item \(\int e^{ax} \dd{x} = \frac{1}{a} e^{ax} + C\)
\item \(\int x e^{ax} \dd{x} = \frac{1}{a^2} (ax-1) e^{ax} + C\)
\item \(\int x^n e^{ax} \dd{x} = \frac{1}{a} x^n e^{ax} - \frac{n}{a} \int x^{n-1} e^{ax} \dd{x}\)
\item \(\int x a^x \dd{x} = \frac{x}{\ln a} a^x - \frac{1}{\ln^2 a} a^x + C\)
\item \(\int x^n a^x \dd{x}
= \frac{1}{\ln a} x^n a^x - \frac{n}{\ln a} \int x^{n-1} a^x \dd{x}\)
\item \(\int e^{ax} \sin bx \dd{x}
= \frac{1}{a^2+b^2} e^{ax} (a \sin bx - b \cos bx) + C\)
\item \(\int e^{ax} \cos bx \dd{x}
= \frac{1}{a^2+b^2} e^{ax} (b \sin bx + a \cos bx) + C\)
\item \(\int e^{ax} \sin^n bx \dd{x}
= \frac{1}{a^2+b^2n^2} e^{ax} \sin^{n-1}bx (a \sin bx - nb \cos bx)
+ \frac{n(n-1)b^2}{a^2+b^2n^2} \int e^{ax} \sin^{n-2}bx \dd{x}\)
\item \(\int e^{ax} \cos^n bx \dd{x}
= \frac{1}{a^2+b^2n^2} e^{ax} \cos^{n-1}bx (a \cos bx + nb \sin bx)
+ \frac{n(n-1)b^2}{a^2+b^2n^2} \int e^{ax} \cos^{n-2}bx \dd{x}\)

\section*{含有对数函数的积分}
\item \(\int \ln x \dd{x} = x \ln x - x + C\)
\item \(\int \frac{\dd{x}}{x \ln x} = \ln\abs{\ln x} + C\)
\item \(\int x^n \ln x \dd{x}
= \frac{1}{n+1} x^{n+1} \left(\ln x - \frac{1}{n+1}\right) + C\)
\item \(\int \ln^n x \dd{x}
= x \ln^n x - n \int \ln^{n-1} x \dd{x}\)
\item \(\int x^m \ln^n x \dd{x}
= \frac{1}{m+1} x^{m+1} \ln^n x - \frac{n}{m+1} \int x^m \ln^{n-1} x \dd{x}\)

\section*{含有双曲函数的积分}
\item \(\int \sinh x \dd{x} = \cosh x + C\)
\item \(\int \cosh x \dd{x} = \sinh x + C\)
\item \(\int \tanh x \dd{x} = \ln\cosh x + C\)
\item \(\int \sinh^2 x \dd{x} = -\frac{x}{2} + \frac{1}{4} \sinh2x + C\)
\item \(\int \cosh^2 x \dd{x} = \frac{x}{2} + \frac{1}{4} \sinh 2x + C\)
\end{enumerate}
